rewrite with definitions.

Syntax.thy
@@ -67,7 +67,7 @@ using push_intro
 by fast
 
 
-fun uncapPred :: "('b::state) \<Rightarrow> 'b set \<Rightarrow> 'b set" where
+definition uncapPred :: "('b::state) \<Rightarrow> 'b set \<Rightarrow> 'b set" where
 "uncapPred s P = {push m s |m. m \<in> P}"
 
 lemma uncapPred_intro:
@@ -76,47 +76,49 @@ proof
   have "m = push (SOME x. m = push x s) s" for m
     using push_intro[of m s] someI_ex by fast
   thus "P = uncapPred s {SOME x. m = push x s |m. m \<in> P}"
-    by auto
+    unfolding uncapPred_def by auto
 qed
 
-fun capPred :: "('b::state) set \<Rightarrow> 'b set" where
+definition capPred :: "('b::state) set \<Rightarrow> 'b set" where
 "capPred P = {popl m |m. m \<in> P}"
 
 
-fun capBeh :: "('b::state) rel \<Rightarrow> 'b rel" where
+definition capBeh :: "('b::state) rel \<Rightarrow> 'b rel" where
 "capBeh b = {(popl m,popl m') |m m'. (m,m') \<in> b}" 
 
-fun uncapBeh :: "('b::state) \<Rightarrow> 'b rel \<Rightarrow> 'b rel" where
+definition uncapBeh :: "('b::state) \<Rightarrow> 'b rel \<Rightarrow> 'b rel" where
 "uncapBeh s b = {(push m s,push m' s') |m m' s'. (m,m') \<in> b}" 
 
 
 (* captures and hides the local effects of a basic. 
 goes from local to global.  *)
-fun capBasic :: "('a,'b::state) basic \<Rightarrow> ('a,'b) basic" where
-"capBasic \<alpha> = (tag \<alpha>, capPred (vc \<alpha>), capBeh (beh \<alpha>))"
+abbreviation capBasic :: "('a,'b::state) basic \<Rightarrow> ('a,'b) basic" where
+"capBasic \<alpha> \<equiv> (tag \<alpha>, capPred (vc \<alpha>), capBeh (beh \<alpha>))"
 
 (* uncaptures and makes visible the effects of a basic. 
 goes from global to local context. *)
-fun uncapBasic :: "('b::state) \<Rightarrow> ('a,'b) basic \<Rightarrow> ('a,'b) basic" where
-"uncapBasic s \<alpha> = (tag \<alpha>, uncapPred s (vc \<alpha>), uncapBeh s (beh \<alpha>))"
+abbreviation uncapBasic :: "('b::state) \<Rightarrow> ('a,'b) basic \<Rightarrow> ('a,'b) basic" where
+"uncapBasic s \<alpha> \<equiv> (tag \<alpha>, uncapPred s (vc \<alpha>), uncapBeh s (beh \<alpha>))"
 
-fun capRely :: "('b::state) rel \<Rightarrow> 'b rel" where
+definition capRely :: "('b::state) rel \<Rightarrow> 'b rel" where
 "capRely R = {(popl m, popl m') |m m'. (m,m') \<in> R}"
 
-fun uncapRely :: "('b::state) rel \<Rightarrow> 'b rel" where
+definition uncapRely :: "('b::state) rel \<Rightarrow> 'b rel" where
 "uncapRely R = {(push m s, push m' s) |m m' s. (m,m') \<in> R}"
 
-fun uncapGuar :: "('b::state) rel \<Rightarrow> 'b rel" where
+definition uncapGuar :: "('b::state) rel \<Rightarrow> 'b rel" where
 "uncapGuar G = {(push m s, push m' s') |m m' s s'. (m,m') \<in> G}"
 
-fun capGuar :: "('b::state) rel \<Rightarrow> 'b rel" where
-"capGuar G = {(popl m, popl m') |m m'. (m,m') \<in> G}"
-
+abbreviation (input) capGuar :: "('b::state) rel \<Rightarrow> 'b rel" where
+"capGuar G \<equiv> capBeh G"
+lemmas capGuar_def = capBeh_def
 
 lemma cap_uncapBeh [simp]: "capBeh (uncapBeh s b) = b"
+unfolding capBeh_def uncapBeh_def
 by (auto, metis popl_push)
 
 lemma cap_uncapPred [simp]: "capPred (uncapPred s P) = P"
+unfolding capPred_def uncapPred_def
 by (auto, metis popl_push)
 
 lemma cap_uncapBasic [simp]: "capBasic (uncapBasic s \<alpha>) = \<alpha>"
@@ -128,46 +130,69 @@ lemma uncap_capBasic: "uncapBasic s (capBasic \<alpha>) = \<alpha>"
 oops
 
 lemma uncap_capGuar [simp]: "uncapGuar (capGuar G) = G"
+unfolding capGuar_def uncapGuar_def
 by auto (metis (full_types) popr_push push_intro)+
 
 lemma cap_uncapGuar [simp]: "capGuar (uncapGuar G) = G"
+unfolding capGuar_def uncapGuar_def
 by auto (metis (full_types) popr_push push_intro)+
+
+lemma uncapBeh_in_uncapGuar: "uncapBeh s G \<subseteq> uncapGuar G"
+unfolding uncapBeh_def uncapGuar_def by fast
+
+(* lemma capBeh_in_capGuar: "capBeh G \<subseteq> capGuar G"
+unfolding capBeh_def capGuar_def by simp *)
 
 
 lemma capPred_mono [simp]: "P \<subseteq> P' \<Longrightarrow> capPred P \<subseteq> capPred P'"
-by auto
+unfolding capPred_def uncapPred_def by auto
 
 lemma uncapGuar_mono [simp]: "G \<subseteq> G' \<Longrightarrow> (uncapGuar G \<subseteq> uncapGuar G')"
-by auto
+unfolding capGuar_def uncapGuar_def by auto
+
 lemma capGuar_mono [simp]: "G \<subseteq> G' \<Longrightarrow> capGuar G \<subseteq> capGuar G'"
-by auto
+unfolding capGuar_def uncapGuar_def by auto
+
 lemma uncapGuar_capPred: "Id_on G \<subseteq> uncapGuar (Id_on (capPred G))"
 proof -
   have "G \<subseteq> {push m s |m s. m \<in> capPred G}"
-    by clarsimp (metis popl_push push_intro)
-  thus ?thesis using Id_on_eqI by clarsimp blast
+    unfolding capPred_def by clarsimp (metis popl_push push_intro)
+  thus ?thesis using Id_on_eqI 
+    unfolding uncapGuar_def by clarsimp blast
 qed
+
+lemma capPred_in_capGuar: "m \<in> capPred G \<Longrightarrow> (m,m) \<in> capGuar (Id_on G)"
+unfolding capGuar_def capPred_def by auto
 
 lemma uncapGuar_eq [simp]: "(uncapGuar G \<subseteq> uncapGuar G') = (G \<subseteq> G')"
 by (metis capGuar_mono cap_uncapGuar uncapGuar_mono)
 
 
 lemma capGuar_relcomp [simp]: "capGuar (G O G') = capGuar G O capGuar G'"
+unfolding capGuar_def
 by auto (metis (mono_tags) popr_push push_intro relcomp.simps)
 
 lemma uncapGuar_relcomp [simp]: "uncapGuar (G O G') = uncapGuar G O uncapGuar G'"
+unfolding uncapGuar_def
 by (auto, blast, metis popl_push relcomp.relcompI)
 
 
 lemma capPred_inter [simp]: "capPred (P \<inter> P') = capPred P \<inter> capPred P'"
+unfolding capPred_def
 by auto (metis popl_push push_intro)
 
 lemma uncapGuar_inter [simp]: "uncapGuar (G \<inter> G') = uncapGuar G \<inter> uncapGuar G'"
+unfolding uncapGuar_def
 by auto (metis (full_types) popr_push push_intro)
+
+lemma capPred_empty [simp]: "capPred {} = {}"
+unfolding capPred_def by simp
+lemma uncapPred_empty [simp]: "uncapPred s {} = {}"
+unfolding uncapPred_def by simp
 
 
 lemma stable_uncap: "stable (uncapRely R) (uncapPred s P) \<Longrightarrow> stable R P"
-unfolding stable_def
+unfolding stable_def uncapRely_def uncapPred_def
 by (auto, metis popl_push)
 
 
