Rules.thy
@@ -158,9 +158,7 @@ next
   case (Capture s c)
   have "guar\<^sub>\<alpha> (capBasic \<beta>) G \<Longrightarrow> guar\<^sub>\<alpha> \<beta> (uncapGuar G)"
     if "\<beta> \<in> basics c" for \<beta> using guar_capE cap_uncapGuar by blast
-  hence "\<forall>\<beta>\<in>basics c. guar\<^sub>\<alpha> \<beta> (uncapGuar G)"
-    using Capture(3) by simp
-  thus ?case using Capture(1,2) by (simp add: rules.capture)
+  thus ?case using Capture by (simp add: rules.capture)  
 qed (auto)
 
 lemma seq_rot:
